wp and proof rules

src/Iris/Examples/IProp.lean
@@ -70,7 +70,7 @@ class abbrev HasPointsToF1 (γ : GName) (GF : outParam _) (F : outParam (Type _)
     [UFraction F] := ElemG GF (F1 (F := F))
 
 /- Define notation for the heap. -/
-def points_to (γ : GName) [HasPointsToF1 γ GF F] (k : Nat) (v : String) :=
+def points_to (γ : GName) [HasPointsToF1 γ GF F] (k : Nat) (v : String) : IProp GF :=
   iOwn (GF := GF) (F := F1 (F := F)) γ (Frag k (own one) (toAgree ⟨v⟩))
 
 notation k:50 " ↦[" γ:50 "] " v:50 => points_to γ k v
@@ -87,5 +87,114 @@ example {γ : GName} : 5 ↦[γ] "A" ∗ 5 ↦[γ] "B" ⊢ False := by
   grind
 
 end Example2
+
+/-! Example: a typical step-indexed weakest precondition -/
+section Example3
+
+open OFE
+
+/- In this example, we are given a type of expressions and a type of states, as well as a
+   single-stepping function from an operational semantics. -/
+class OperationalSemantics (Expr State Value : Type _) where
+  step : Expr × State → Expr × State
+  to_value : Expr → Option Value
+export OperationalSemantics (step to_value)
+variable (Expr State Value : Type _) [OperationalSemantics Expr State Value]
+
+/- Let's say that we are also given two OFunctors, and an interpretation of the state into
+   state using these resources. -/
+variable (F3 F4 : OFunctorPre) [RFunctorContractive F3] [RFunctorContractive F4]
+variable {GF} [ElemG GF F3] [ElemG GF F4]
+class StateInterpretation (State : Type _) (GF : BundledGFunctors) where
+  state_interp : State → IProp GF
+export StateInterpretation (state_interp)
+variable [StateInterpretation State GF]
+
+/- Again, doing this trick so that we can write WP notations that don't explicitly include
+   Expr State and Value. -/
+set_option synthInstance.checkSynthOrder false in
+class abbrev Ex3WP {Expr : Type _} {State Value : outParam (Type _)} {GF : outParam BundledGFunctors} :=
+  OperationalSemantics Expr State Value,
+  StateInterpretation State GF
+
+/- Now, we can define a contractive functor for the weakest precondition. -/
+def wp_F (wp : Expr → (Value → IProp GF) → IProp GF) (e : Expr) (Φ : Value → IProp GF) :
+    IProp GF := iprop(
+  (∃ v : Value, ⌜@to_value _ State _ _ e = some v⌝ ∗ |==> Φ v) ∨
+  ∀ s, @state_interp State _ _ s -∗
+    ∃ e' s', ⌜@step _ _ Value _ (e, s) = (e', s') ⌝ ∗ ▷ |==> (@state_interp _ _ _  s' ∗ wp e' Φ))
+
+instance wp_F_contractive : Contractive (@wp_F Expr State Value _ GF _) where
+  distLater_dist {n x y HL} e Φ := by
+    refine or_ne.ne (.of_eq rfl) ?_
+    refine forall_ne (fun _ => ?_)
+    refine wand_ne.ne (.of_eq rfl) ?_
+    refine exists_ne (fun v => ?_)
+    refine exists_ne (fun _ => ?_)
+    refine sep_ne.ne (.of_eq rfl) ?_
+    refine Contractive.distLater_dist fun m Hm => ?_
+    refine BIUpdate.bupd_ne.ne ?_
+    refine sep_ne.ne (.of_eq rfl) ?_
+    exact HL m Hm v Φ
+
+def wp {Expr State Value : Type _} [@Ex3WP Expr State Value GF] (e : Expr) (Φ : Value → IProp GF) : IProp GF :=
+  (fixpoint <| @wp_F Expr State Value _ GF _) e Φ
+
+theorem wp_unfold (e : Expr) (Φ : Value → IProp GF) :
+    wp e Φ ≡ iprop(
+        (∃ v : Value, ⌜@to_value _ State _ _ e = some v⌝ ∗ |==> Φ v) ∨
+        ∀ s, @state_interp State _ _ s -∗
+          ∃ e' s', ⌜@step _ _ Value _ (e, s) = (e', s') ⌝ ∗
+          ▷ |==> (@state_interp _ _ _  s' ∗ wp e' Φ)) := by
+  apply fixpoint_unfold (f := ⟨(@wp_F Expr State Value _ GF _),
+                                @OFE.ne_of_contractive _ _ _ _ (@wp_F Expr State Value _ GF _) _⟩)
+
+/- Now, we can derive some example proof rules. First let's prove a rule for pure deterministic steps: -/
+example (e e' : Expr) Φ (Hstep : ∀ {s : State}, @step _ _ Value _ (e, s) = (e', s)) :
+    wp e' Φ ⊢ wp e Φ := by
+  refine .trans ?_ (equiv_iff.mp (@wp_unfold Expr State Value _ GF _ _ _).symm).mp
+  iintro Hspec
+  iright
+  iintro %s Hs
+  iexists e', s
+  isplitr
+  · ipure_intro
+    exact Hstep
+  · refine .trans ?_ later_intro      -- FIXME: once iNext is implemented
+    refine .trans ?_ BIUpdate.intro   -- FIXME: once iModIntro is implemented
+    iintro ⟨Hspec, Hs⟩
+    isplitl [Hs]
+    · iexact Hs
+    · iexact Hspec
+
+/- The pattern of rules for stateful steps, for example, writing to a piece of memory.
+   This style of rule applies when ownership over a resource P (eg. k ↦[γ] v) ensures that the state
+   can step the expression e to some new expression e', and can be updated to a new resource P'
+   in the stepped-to state.
+   Then, it suffies to have access to P, and show that access to P' is enough to verify e'. -/
+example (e e' : Expr) (P P' : IProp GF) Φ
+      (Hstep : ∀ s, iprop(P ∗ @state_interp State GF _ s ⊢ ∃ s',
+          ⌜@step _ _ Value _ (e, s) = (e', s')⌝ ∗ |==> (P' ∗ @state_interp State GF _ s'))) :
+    P ∗ (P' -∗ wp e' Φ) ⊢ wp e Φ := by
+  refine .trans ?_ (equiv_iff.mp (@wp_unfold Expr State Value _ GF _ _ _).symm).mp
+  iintro ⟨HP, Hspec⟩
+  iright
+  iintro %s Hs
+  istop -- FIXME: iHave bug?
+  refine .trans (sep_mono (sep_mono (wand_intro (Hstep s)) .rfl) .rfl) ?_
+  iintro ⟨⟨Hcont, Hspec⟩, HP⟩
+  icases Hcont $$ HP with ⟨%s', %Hstep, Hupd⟩
+  iexists e', s'
+  isplitr
+  · ipure_intro; exact Hstep
+  refine .trans ?_ later_intro   -- FIXME: once iNext is implemented
+  refine .trans bupd_frame_l ?_  -- FIXME: once iMod is implemented
+  refine BIUpdate.mono ?_        -- FIXME: once iMod is implemented
+  iintro ⟨Hspec, HP', Hs⟩
+  isplitl [Hs]
+  · iexact Hs
+  · iapply Hspec $$ HP'
+
+end Example3
 
 end Iris.Examples
